rename data structures

Orderedtree/DTreeMap/Basic.lean
@@ -3,7 +3,7 @@ Copyright (c) 2024 Lean FRO, LLC. All rights reserved.
 Released under Apache 2.0 license as described in the file LICENSE.
 Authors: Markus Himmel
 -/
-import Orderedtree.DOrderedTree.Internal.Impl
+import Orderedtree.DTreeMap.Internal.Impl
 
 set_option autoImplicit false
 set_option linter.missingDocs true
@@ -15,36 +15,36 @@ variable {α : Type u} {β : α → Type v} {cmp : α → α → Ordering}
 namespace Std
 
 /-- Binary search trees. -/
-structure DOrderedTree (α : Type u) (β : α → Type v) (cmp : α → α → Ordering) where
+structure DTreeMap (α : Type u) (β : α → Type v) (cmp : α → α → Ordering) where
   /-- Internal implementation detail of the binary search tree. -/
-  inner : DOrderedTree.Internal.Impl α β
+  inner : DTreeMap.Internal.Impl α β
   /-- Internal implementation detail of the binary search tree. -/
   wf : letI : Ord α := ⟨cmp⟩; inner.WF
 
-namespace DOrderedTree
+namespace DTreeMap
 
 @[inline]
-def isEmpty (t : DOrderedTree α β cmp) : Bool :=
+def isEmpty (t : DTreeMap α β cmp) : Bool :=
   t.inner.isEmpty
 
 /-- Creates a new empty binary search tree. -/
 @[inline]
-def empty : DOrderedTree α β cmp :=
+def empty : DTreeMap α β cmp :=
   letI : Ord α := ⟨cmp⟩; ⟨Internal.Impl.empty, .empty⟩
 
 /-- Inserts the mapping `(a, b)` into the binary search tree. -/
 @[inline]
-def insert (l : DOrderedTree α β cmp) (a : α) (b : β a) : DOrderedTree α β cmp :=
+def insert (l : DTreeMap α β cmp) (a : α) (b : β a) : DTreeMap α β cmp :=
   letI : Ord α := ⟨cmp⟩; ⟨(l.inner.insert a b l.wf.balanced).impl, .insert l.wf⟩
 
 /-- Returns `true` if the given key is present in the map. -/
 @[inline]
-def contains (l : DOrderedTree α β cmp) (a : α) : Bool :=
+def contains (l : DTreeMap α β cmp) (a : α) : Bool :=
   letI : Ord α := ⟨cmp⟩; l.inner.contains a
 
-instance : Membership α (DOrderedTree α β cmp) where
+instance : Membership α (DTreeMap α β cmp) where
   mem m a := m.contains a
 
-end DOrderedTree
+end DTreeMap
 
 end Std
