Orderedtree/TreeMap/Raw.lean
@@ -3,7 +3,7 @@ Copyright (c) 2024 Lean FRO, LLC. All rights reserved.
 Released under Apache 2.0 license as described in the file LICENSE.
 Authors: Markus Himmel
 -/
-import Orderedtree.DOrderedTree.Raw
+import Orderedtree.DTreeMap.Raw
 
 set_option autoImplicit false
 set_option linter.missingDocs true
@@ -14,16 +14,16 @@ variable {α : Type u} {β : Type v} {cmp : α → α → Ordering}
 
 namespace Std
 
-namespace OrderedTree
+namespace TreeMap
 
-@[inherit_doc DOrderedTree.Raw]
+@[inherit_doc DTreeMap.Raw]
 structure Raw (α : Type u) (β : Type v) (cmp : α → α → Ordering) where
   /-- Internal implementation detail of the binary search tree. -/
-  inner : DOrderedTree.Raw α (fun _ => β) cmp
+  inner : DTreeMap.Raw α (fun _ => β) cmp
 
 namespace Raw
 
-@[inherit_doc DOrderedTree.Raw.WF]
+@[inherit_doc DTreeMap.Raw.WF]
 structure WF (l : Raw α β cmp) where
   /-- Internal implementation detail of the binary search tree. -/
   out : l.inner.WF
@@ -31,23 +31,23 @@ structure WF (l : Raw α β cmp) where
 instance {t : Raw α β cmp} : Coe t.WF t.inner.WF where
   coe t := t.out
 
-@[inline, inherit_doc DOrderedTree.Raw.empty]
+@[inline, inherit_doc DTreeMap.Raw.empty]
 def empty : Raw α β cmp :=
-  ⟨DOrderedTree.Raw.empty⟩
+  ⟨DTreeMap.Raw.empty⟩
 
-@[inline, inherit_doc DOrderedTree.Raw.isEmpty]
+@[inline, inherit_doc DTreeMap.Raw.isEmpty]
 def isEmpty (t : Raw α β cmp) : Bool :=
   t.inner.isEmpty
 
-@[inline, inherit_doc DOrderedTree.Raw.insert]
+@[inline, inherit_doc DTreeMap.Raw.insert]
 def insert (l : Raw α β cmp) (a : α) (b : β) : Raw α β cmp :=
   ⟨l.inner.insert a b⟩
 
-@[inline, inherit_doc DOrderedTree.Raw.insertFast]
+@[inline, inherit_doc DTreeMap.Raw.insertFast]
 def insertFast (l : Raw α β cmp) (h : l.WF) (a : α) (b : β) : Raw α β cmp :=
   ⟨l.inner.insertFast h.out a b⟩
 
-@[inline, inherit_doc DOrderedTree.Raw.contains]
+@[inline, inherit_doc DTreeMap.Raw.contains]
 def contains (l : Raw α β cmp) (a : α) : Bool :=
   l.inner.contains a
 
@@ -56,6 +56,6 @@ instance : Membership α (Raw α β cmp) where
 
 end Raw
 
-end OrderedTree
+end TreeMap
 
 end Std
