Orderedtree/TreeSet/Basic.lean
@@ -3,7 +3,7 @@ Copyright (c) 2024 Lean FRO, LLC. All rights reserved.
 Released under Apache 2.0 license as described in the file LICENSE.
 Authors: Markus Himmel
 -/
-import Orderedtree.OrderedTree.Basic
+import Orderedtree.TreeMap.Basic
 
 set_option autoImplicit false
 set_option linter.missingDocs true
@@ -14,31 +14,31 @@ variable {α : Type u} {cmp : α → α → Ordering}
 
 namespace Std
 
-structure OrderedSet (α : Type u) (cmp : α → α → Ordering) where
+structure TreeSet (α : Type u) (cmp : α → α → Ordering) where
   /-- Internal implementation detail of the binary search tree. -/
-  inner : OrderedTree α Unit cmp
+  inner : TreeMap α Unit cmp
 
-namespace OrderedSet
-
-@[inline]
-def empty : OrderedSet α cmp :=
-  ⟨OrderedTree.empty⟩
+namespace TreeSet
 
 @[inline]
-def isEmpty (t : OrderedSet α cmp) : Bool :=
+def empty : TreeSet α cmp :=
+  ⟨TreeMap.empty⟩
+
+@[inline]
+def isEmpty (t : TreeSet α cmp) : Bool :=
   t.inner.isEmpty
 
 @[inline]
-def insert (l : OrderedSet α cmp) (a : α) : OrderedSet α cmp :=
+def insert (l : TreeSet α cmp) (a : α) : TreeSet α cmp :=
   ⟨l.inner.insert a ()⟩
 
 @[inline]
-def contains (l : OrderedSet α cmp) (a : α) : Bool :=
+def contains (l : TreeSet α cmp) (a : α) : Bool :=
   l.inner.contains a
 
-instance : Membership α (OrderedSet α cmp) where
+instance : Membership α (TreeSet α cmp) where
   mem m a := m.contains a
 
-end OrderedSet
+end TreeSet
 
 end Std
