Orderedtree/DTreeMap/Internal/Impl.lean
@@ -4,8 +4,8 @@ Released under Apache 2.0 license as described in the file LICENSE.
 Authors: Markus Himmel
 -/
 import Orderedtree.Classes.LawfulEqOrd
-import Orderedtree.DOrderedTree.Internal.Impl.Attr
-import Orderedtree.DOrderedTree.Internal.Impl.Operations
+import Orderedtree.DTreeMap.Internal.Impl.Attr
+import Orderedtree.DTreeMap.Internal.Impl.Operations
 import Orderedtree.Classes.TransOrd
 import Lean.Elab.Tactic
 
@@ -22,7 +22,7 @@ universe u v w
 
 variable {α : Type u} {β : α → Type v} {γ : α → Type w} {δ : Type w} {m : Type w → Type w}
 
-namespace Std.DOrderedTree.Internal
+namespace Std.DTreeMap.Internal
 
 namespace Impl
 
@@ -56,7 +56,7 @@ theorem WF.balanced [Ord α] {t : Impl α β} : WF t → t.Balanced
 
 end Impl
 
-end Std.DOrderedTree.Internal
+end Std.DTreeMap.Internal
 
 -- open Lean
 
@@ -66,7 +66,7 @@ end Std.DOrderedTree.Internal
 --   let mut unknown : Array Name := #[]
 --   let mut totalSize : Nat := 0
 --   for (name, info) in env.constants do
---     if (`Std.DOrderedTree.Internal.Impl).isPrefixOf name then
+--     if (`Std.DTreeMap.Internal.Impl).isPrefixOf name then
 --       if let some e := info.value? then
 --         let numObjs ← e.numObjs
 --         arr := arr.push (numObjs, (name, m!"{info.type}"))
