Orderedtree/TreeSet/RawLemmas.lean
@@ -3,11 +3,11 @@ Copyright (c) 2024 Lean FRO, LLC. All rights reserved.
 Released under Apache 2.0 license as described in the file LICENSE.
 Authors: Markus Himmel
 -/
-import Orderedtree.OrderedTree.RawLemmas
-import Orderedtree.OrderedSet.Raw
+import Orderedtree.TreeMap.RawLemmas
+import Orderedtree.TreeSet.Raw
 
 /-!
-# API lemmas for `OrderedTree.Raw`
+# API lemmas for `TreeMap.Raw`
 -/
 
 set_option linter.missingDocs true
@@ -15,33 +15,33 @@ set_option autoImplicit false
 
 universe u v
 
-namespace Std.OrderedSet.Raw
+namespace Std.TreeSet.Raw
 
 attribute [local instance] TransOrd.ofTransCmp
 
-variable {α : Type u} {β : Type v} {cmp : α → α → Ordering} {t : OrderedSet.Raw α cmp}
+variable {α : Type u} {β : Type v} {cmp : α → α → Ordering} {t : TreeSet.Raw α cmp}
 
-theorem isEmpty_empty : (empty : OrderedSet.Raw α cmp).isEmpty :=
-  OrderedTree.Raw.isEmpty_empty
+theorem isEmpty_empty : (empty : TreeSet.Raw α cmp).isEmpty :=
+  TreeMap.Raw.isEmpty_empty
 
 theorem mem_iff_contains {k : α} : k ∈ t ↔ t.contains k :=
-  OrderedTree.Raw.mem_iff_contains
+  TreeMap.Raw.mem_iff_contains
 
 theorem contains_congr [TransCmp cmp] (h : t.WF) {k k' : α} (hab : cmp k k' == .eq) :
     t.contains k = t.contains k' :=
-  OrderedTree.Raw.contains_congr h hab
+  TreeMap.Raw.contains_congr h hab
 
 theorem mem_congr [TransCmp cmp] (h : t.WF) {k k' : α} (hab : cmp k k' == .eq) : k ∈ t ↔ k' ∈ t :=
-  OrderedTree.Raw.mem_congr h hab
+  TreeMap.Raw.mem_congr h hab
 
-theorem contains_empty {k : α} : (empty : OrderedSet.Raw α cmp).contains k = false :=
-  OrderedTree.Raw.contains_empty
+theorem contains_empty {k : α} : (empty : TreeSet.Raw α cmp).contains k = false :=
+  TreeMap.Raw.contains_empty
 
-theorem mem_empty {k : α} : k ∉ (empty : OrderedSet.Raw α cmp) :=
-  OrderedTree.Raw.mem_empty
+theorem mem_empty {k : α} : k ∉ (empty : TreeSet.Raw α cmp) :=
+  TreeMap.Raw.mem_empty
 
 theorem contains_insert [h : TransCmp cmp] (h : t.WF) {k a : α} :
     (t.insert k).contains a = (cmp k a == .eq || t.contains a) :=
-  OrderedTree.Raw.contains_insert h
+  TreeMap.Raw.contains_insert h
 
-end Std.OrderedSet.Raw
+end Std.TreeSet.Raw
